.

GIT.v
@@ -8,6 +8,8 @@ Require Export Lia.
 
 Module Preliminaries.
 
+  Import ListNotations.
+
   Section NaturalNumber.
 
     Lemma div_mod_property :
@@ -488,6 +490,17 @@ Module Preliminaries.
 
   End Ensembles.
 
+  Section Lists.
+    
+    Fixpoint lookup {A : Type} {B : Type} (eq_A_dec : forall x1 : A, forall x2 : A, {x1 = x2} + {x1 <> x2}) (x : A) (ps : list (A * B)) : option B :=
+      match ps with
+      | [] => None
+      | (x1, y1) :: ps2 => if eq_A_dec x x1 then Some y1 else lookup eq_A_dec x ps2
+      end
+    .
+
+  End Lists.
+
 End Preliminaries.
 
 Module The_General_Idea_Behind_Goedel's_Proof.
@@ -500,7 +513,6 @@ Module The_General_Idea_Behind_Goedel's_Proof.
 
     Class GoedelianLanguage (E : Type) : Type :=
       { enumE : nat -> E
-      ; eq_E_dec : forall e1 : E, forall e2 : E, {e1 = e2} + {e1 <> e2}
       ; E_is_denumerable : forall e : E, {n : nat | enumE n = e}
       ; isSentence : Ensemble E
       ; isProvable : Ensemble E
@@ -1067,3 +1079,133 @@ Module The_General_Idea_Behind_Goedel's_Proof.
   End Exercise.
 
 End The_General_Idea_Behind_Goedel's_Proof.
+
+Module Tarski's_Theorem_for_Arithmetic.
+
+  Import Preliminaries.
+
+  Import The_General_Idea_Behind_Goedel's_Proof.
+
+  Section The_Language_L_E.
+
+    Definition Var : Set :=
+      nat
+    .
+
+    Definition Val : Type :=
+      nat
+    .
+
+    Definition Assignment : Type :=
+      Var -> Val
+    .
+
+    Inductive Term : Set :=
+    | IVar : forall i1 : Var, Term
+    | Zero : Term
+    | Succ : forall t1 : Term, Term
+    | Plus : forall t1 : Term, forall t2 : Term, Term
+    | Mult : forall t1 : Term, forall t2 : Term, Term
+    | Expo : forall t1 : Term, forall t2 : Term, Term
+    .
+
+    Fixpoint getFVs_Term (t : Term) : Ensemble Var :=
+      match t with
+      | IVar i1 => singleton i1
+      | Zero => empty
+      | Succ t1 => getFVs_Term t1
+      | Plus t1 t2 => union (getFVs_Term t1) (getFVs_Term t2)
+      | Mult t1 t2 => union (getFVs_Term t1) (getFVs_Term t2)
+      | Expo t1 t2 => union (getFVs_Term t1) (getFVs_Term t2)
+      end
+    .
+
+    Fixpoint applySubst_Term (theta : list (Var * Term)) (t : Term) : Term :=
+      match t with
+      | IVar i1 =>
+        match lookup Nat.eq_dec i1 theta with
+        | None => IVar i1
+        | Some t' => t'
+        end
+      | Zero => Zero
+      | Succ t1 => Succ (applySubst_Term theta t1)
+      | Plus t1 t2 => Plus (applySubst_Term theta t1) (applySubst_Term theta t2)
+      | Mult t1 t2 => Mult (applySubst_Term theta t1) (applySubst_Term theta t2)
+      | Expo t1 t2 => Expo (applySubst_Term theta t1) (applySubst_Term theta t2)
+      end
+    .
+
+    Fixpoint evalTerm (v : Assignment) (t : Term) : Val :=
+      match t with
+      | IVar i1 => v i1
+      | Zero => 0
+      | Succ t1 => S (evalTerm v t1)
+      | Plus t1 t2 => evalTerm v t1 + evalTerm v t2
+      | Mult t1 t2 => evalTerm v t1 * evalTerm v t2
+      | Expo t1 t2 => (evalTerm v t1)^(evalTerm v t2)
+      end
+    .
+
+    Inductive Formula : Set :=
+    | Eqn : forall t1 : Term, forall t2 : Term, Formula
+    | Leq : forall t1 : Term, forall t2 : Term, Formula
+    | Neg : forall f1 : Formula, Formula
+    | Imp : forall f1 : Formula, forall f2 : Formula, Formula
+    | All : forall i1 : Var, forall f2 : Formula, Formula
+    .
+
+    Fixpoint getFVs_Formula (f : Formula) : Ensemble Var :=
+      match f with
+      | Eqn t1 t2 => union (getFVs_Term t1) (getFVs_Term t2)
+      | Leq t1 t2 => union (getFVs_Term t1) (getFVs_Term t2)
+      | Neg f1 => getFVs_Formula f1
+      | Imp f1 f2 => union (getFVs_Formula f1) (getFVs_Formula f2)
+      | All i1 f2 => delete i1 (getFVs_Formula f2)
+      end
+    .
+
+    Fixpoint applySubst_Formula (theta : list (Var * Term)) (f : Formula) : Formula :=
+      match f with 
+      | Eqn t1 t2 => Eqn (applySubst_Term theta t1) (applySubst_Term theta t2)
+      | Leq t1 t2 => Leq (applySubst_Term theta t1) (applySubst_Term theta t2)
+      | Neg f1 => Neg (applySubst_Formula theta f1)
+      | Imp f1 f2 => Imp (applySubst_Formula theta f1) (applySubst_Formula theta f2)
+      | All i1 f2 => All i1 (applySubst_Formula (filter (fun pair : (Var * Term) => if Nat.eq_dec (fst pair) i1 then true else false) theta) f2)
+      end
+    .
+
+    Fixpoint evalFormula (v : Assignment) (f : Formula) : Prop :=
+      match f with
+      | Eqn t1 t2 => evalTerm v t1 = evalTerm v t2
+      | Leq t1 t2 => evalTerm v t1 <= evalTerm v t2
+      | Neg f1 => ~ evalFormula v f1
+      | Imp f1 f2 => evalFormula v f1 -> evalFormula v f2
+      | All i1 f2 => forall n : Val, evalFormula (fun i : Var => if Nat.eq_dec i i1 then n else v i) f2
+      end
+    .
+  
+    Class isExpr (E : Set) : Type :=
+      { getFVs : E -> Ensemble Var
+      ; applySubst : list (Var * Term) -> E -> E
+      }
+    .
+
+    Definition isClosed {E : Set} {E_isExpr : isExpr E} (e : E) : Prop :=
+      isSubsetOf (getFVs e) empty
+    .
+
+    Instance isExpr_Term : isExpr Term :=
+      { getFVs := getFVs_Term
+      ; applySubst := applySubst_Term
+      }
+    .
+
+    Instance isExpr_Formula : isExpr Formula :=
+      { getFVs := getFVs_Formula
+      ; applySubst := applySubst_Formula
+      }
+    .
+
+  End The_Language_L_E.
+
+End Tarski's_Theorem_for_Arithmetic.
